Seccompfilter.v
@@ -34,15 +34,19 @@ Fixpoint seccomp_func_filter (f: Seccomp.code) : bool :=
   | Sld_w_len :: rest => seccomp_func_filter rest
   | Sldx_w_len :: rest => seccomp_func_filter rest
 
+  | Sld_imm k :: rest => seccomp_func_filter rest
 (*
   | Sld_mem k :: rest =>
     (Int.unsigned k <? seccomp_memwords) &&
     (seccomp_func_filter rest)
 *)
+
   | Smisc_tax :: rest => seccomp_func_filter rest
   | Smisc_txa :: rest => seccomp_func_filter rest
+
   | Sret_k k :: rest => seccomp_func_filter rest
   | Sret_a :: rest => seccomp_func_filter rest
+
   | _ => false
   end.
 
